Add monad

examples/simple.ml
@@ -2,7 +2,7 @@ module User = struct
   type t = { username : string }
 
   let equal _a _b = false
-    (* String.equal a.username b.username *)
+  (* String.equal a.username b.username *)
 
   let pp ppf v = Format.pp_print_string ppf v.username
 end
@@ -13,11 +13,7 @@ let alice = User.{ username = "Alice" }
 let bob = User.{ username = "Bob" }
 let charlie = User.{ username = "Charlie" }
 let meredith = User.{ username = "Meredith" }
-
-let map =
-  Users.v alice [ bob ]
-  |> Users.add charlie [ meredith; bob ]
-
+let map = Users.v alice [ bob ] |> Users.add charlie [ meredith; bob ]
 let owners = Users.owners map
 let ef = Users.effective_readers map
 
@@ -26,3 +22,20 @@ let () =
   List.iter (Format.printf "%a\n%!" User.pp) owners;
   print_endline "\nEffective Reader Set:";
   List.iter (Format.printf "%a\n%!" User.pp) ef
+
+(* Using Monad like type *)
+
+let map2 = Users.v meredith [ alice ]
+
+let v =
+  let module M = Users.Monad in
+  let open M.Syntax in
+  let* v1 = M.return map "Secret " in
+  let+ v2 = M.return map2 "Data" in
+  v1 ^ v2
+
+let () =
+  print_endline "Owners v:";
+  List.iter
+    (Format.printf "%a\n%!" User.pp)
+    (Users.owners (Users.Monad.label v))
