src/ml/generated/difc_fstar.ml
@@ -1,6 +1,15 @@
 open Prims
 type ('a, 'f) label =
   ('a, ('a, unit) FStar_OrdSet.ordset, unit) FStar_OrdMap.ordmap
+type ('p, 'f, 'm1, 'm2) equal =
+  ('p, ('p, unit) FStar_OrdSet.ordset, unit, unit, unit) FStar_OrdMap.equal
+let v :
+  'p .
+    'p FStar_OrdMap.cmp ->
+      'p -> ('p, unit) FStar_OrdSet.ordset -> ('p, unit) label
+  =
+  fun f ->
+    fun o -> fun v1 -> FStar_OrdMap.update f o v1 (FStar_OrdMap.empty f)
 let owners :
   'p .
     ('p -> 'p -> Prims.bool) ->
@@ -16,7 +25,7 @@ let readers_with_empty :
       fun l ->
         match FStar_OrdMap.select f k l with
         | FStar_Pervasives_Native.None -> FStar_OrdSet.empty f
-        | FStar_Pervasives_Native.Some v -> v
+        | FStar_Pervasives_Native.Some v1 -> v1
 let effective_readers :
   'p .
     ('p -> 'p -> Prims.bool) ->
@@ -55,3 +64,43 @@ let readers_agree :
         fun l2 ->
           FStar_OrdSet.subset f (readers_with_empty f o l1)
             (readers_with_empty f o l2)
+let add :
+  'p .
+    'p FStar_OrdMap.cmp ->
+      'p ->
+        ('p, unit) FStar_OrdSet.ordset ->
+          ('p, unit) label -> ('p, unit) label
+  = fun f -> fun o -> fun v1 -> fun l -> FStar_OrdMap.update f o v1 l
+let join :
+  'p .
+    'p FStar_OrdMap.cmp ->
+      ('p, unit) label -> ('p, unit) label -> ('p, unit) label
+  =
+  fun f ->
+    fun l1 ->
+      fun l2 ->
+        let owners_l1 = owners f l1 in
+        let owners_l2 = owners f l2 in
+        let update_from_label o from_label other_label m =
+          match ((FStar_OrdMap.select f o from_label),
+                  (FStar_OrdMap.select f o other_label))
+          with
+          | (FStar_Pervasives_Native.Some rs, FStar_Pervasives_Native.None)
+              -> add f o rs m
+          | (FStar_Pervasives_Native.Some r1, FStar_Pervasives_Native.Some
+             r2) -> add f o (FStar_OrdSet.intersect f r1 r2) m in
+        let rec fold from_label os other_label macc =
+          match os with
+          | o::[] ->
+              let v1 = update_from_label o from_label other_label macc in v1
+          | o::rest ->
+              let v1 = update_from_label o from_label other_label macc in
+              fold from_label rest other_label v1 in
+        let uu___ =
+          match FStar_OrdMap.choose f l1 with
+          | FStar_Pervasives_Native.Some m -> m in
+        match uu___ with
+        | (choosen_owner, choosen_readers) ->
+            let start = v f choosen_owner choosen_readers in
+            let m1 = fold l1 (FStar_OrdSet.as_list f owners_l1) l2 start in
+            let m2 = fold l2 (FStar_OrdSet.as_list f owners_l2) l1 m1 in m2
