src/ml/generated/difc_fstar_monad.ml
@@ -1,0 +1,59 @@
+open Prims
+type ('a, 'p, 'f) difc_monad =
+  {
+  value: 'a ;
+  label: ('p, unit) Difc_fstar.label }
+let __proj__Mkdifc_monad__item__value :
+  'a 'p . 'p FStar_OrdMap.cmp -> ('a, 'p, unit) difc_monad -> 'a =
+  fun f -> fun projectee -> match projectee with | { value; label;_} -> value
+let __proj__Mkdifc_monad__item__label :
+  'a 'p .
+    'p FStar_OrdMap.cmp ->
+      ('a, 'p, unit) difc_monad -> ('p, unit) Difc_fstar.label
+  =
+  fun f -> fun projectee -> match projectee with | { value; label;_} -> label
+let get_label :
+  'a 'p .
+    'p FStar_OrdMap.cmp ->
+      ('a, 'p, unit) difc_monad -> ('p, unit) Difc_fstar.label
+  = fun f -> fun l -> l.label
+let return :
+  'a 'p .
+    'p FStar_OrdMap.cmp ->
+      ('p, unit) Difc_fstar.label -> 'a -> ('a, 'p, unit) difc_monad
+  = fun f -> fun l -> fun value -> { value; label = l }
+let bind :
+  'a 'b 'c 'p .
+    'p FStar_OrdMap.cmp ->
+      ('a -> ('b, 'p, unit) difc_monad) ->
+        ('a, 'p, unit) difc_monad -> ('b, 'p, unit) difc_monad
+  =
+  fun f ->
+    fun fn ->
+      fun v ->
+        let dm = fn v.value in
+        let v_label = get_label f v in
+        let l' = Difc_fstar.join f v_label dm.label in
+        let res = { value = (dm.value); label = l' } in res
+let map :
+  'a 'b 'c 'p .
+    'p FStar_OrdMap.cmp ->
+      ('a -> 'b) -> ('a, 'p, unit) difc_monad -> ('b, 'p, unit) difc_monad
+  =
+  fun f ->
+    fun fn ->
+      fun v -> let b1 = fn v.value in { value = b1; label = (v.label) }
+let map_pair :
+  'a 'b 'c 'p .
+    'p FStar_OrdMap.cmp ->
+      ('a -> 'b -> 'c) ->
+        ('a, 'p, unit) difc_monad ->
+          ('b, 'p, unit) difc_monad -> ('c, 'p, unit) difc_monad
+  =
+  fun f ->
+    fun fn ->
+      fun v1 ->
+        fun v2 ->
+          let v' = fn v1.value v2.value in
+          let l' = Difc_fstar.join f v1.label v2.label in
+          { value = v'; label = l' }
