src/fstar/difc_fstar.monad.fst
@@ -1,0 +1,43 @@
+module Difc_fstar.Monad
+
+open Difc_fstar
+
+module Map = FStar.OrdMap
+module Set = FStar.OrdSet
+module List = FStar.List.Tot
+
+noeq
+type difc_monad (a : Type) (p : eqtype) (f : Map.cmp p) = {
+  value : a;
+  label : label p f; 
+}
+
+let get_label (#a:Type) (#p:eqtype) (#f:Map.cmp p) (l : difc_monad a p f) = l.label
+
+let return (#a:Type) (#p:eqtype) (#f:Map.cmp p) (l : label p f) (value : a) = { value; label = l }
+
+let bind (#a:Type) (#b:Type) (#c:Type) (#p:eqtype) (#f:Map.cmp p) 
+  (fn : a -> difc_monad b p f) 
+  (v : difc_monad a p f) :
+  res: difc_monad b p f { is_a_restriction (get_label v) (get_label res) } =
+    let dm = fn v.value in
+	let v_label = get_label v in
+	let l' = join v_label dm.label in
+	let res = { value = dm.value; label = l' } in
+    lemma_join_is_a_restriction v_label dm.label;
+	assert (equal (get_label res) (join v_label dm.label));
+	res
+
+let map (#a:Type) (#b:Type) (#c:Type) (#p:eqtype) (#f:Map.cmp p) 
+  (fn : a -> b) 
+  (v : difc_monad a p f) =
+    let b = fn v.value in
+	{ value = b; label = v.label }
+
+let map_pair (#a:Type) (#b:Type) (#c:Type) (#p:eqtype) (#f:Map.cmp p) 
+  (fn : a -> b -> c) 
+  (v1 : difc_monad a p f) 
+  (v2 : difc_monad b p f) =
+  let v' = fn v1.value v2.value in
+  let l' = join v1.label v2.label in
+  { value = v'; label = l' }
